Test/og/DeviceCache.bpl
@@ -22,18 +22,20 @@ function {:inline} Inv(ghostLock: X, currsize: int, newsize: int) : (bool)
     (ghostLock == nil <==> currsize == newsize)
 }
 
-procedure {:yields} {:phase 1} YieldToReadCache({:linear "tid"} tid': X) returns ({:linear "tid"} tid: X)
-requires {:phase 1} Inv(ghostLock, currsize, newsize) && tid' != nil;
-ensures {:phase 1} Inv(ghostLock, currsize, newsize) && tid != nil && tid == tid' && old(currsize) <= currsize;
+procedure {:yields} {:phase 1} YieldToReadCache({:cnst "tid"} tid: X)
+requires {:phase 1} Inv(ghostLock, currsize, newsize) && tid != nil;
+ensures {:phase 1} Inv(ghostLock, currsize, newsize) && old(currsize) <= currsize;
 {
-   tid := tid';
+   yield;
+   assert {:phase 1} Inv(ghostLock, currsize, newsize) && old(currsize) <= currsize;
 }
 
-procedure {:yields} {:phase 1} YieldToWriteCache({:linear "tid"} tid': X) returns ({:linear "tid"} tid: X)
-requires {:phase 1} Inv(ghostLock, currsize, newsize) && ghostLock == tid' && tid' != nil;
-ensures {:phase 1} Inv(ghostLock, currsize, newsize) && ghostLock == tid && tid != nil && tid == tid' && old(currsize) == currsize && old(newsize) == newsize;
+procedure {:yields} {:phase 1} YieldToWriteCache({:cnst "tid"} tid: X)
+requires {:phase 1} Inv(ghostLock, currsize, newsize) && ghostLock == tid && tid != nil;
+ensures {:phase 1} Inv(ghostLock, currsize, newsize) && ghostLock == tid && old(currsize) == currsize && old(newsize) == newsize;
 {
-    tid := tid';
+    yield;
+    assert {:phase 1} Inv(ghostLock, currsize, newsize) && tid != nil && ghostLock == tid && old(currsize) == currsize && old(newsize) == newsize;
 }
 
 procedure Allocate({:linear "tid"} xls': [X]bool) returns ({:linear "tid"} xls: [X]bool, {:linear "tid"} xl: X);
@@ -47,7 +49,8 @@ requires {:phase 1} xls' == mapconstbool(true);
 
     yield;
 
-    call xls := Init(xls');
+    xls := xls';
+    call Init(xls);
     
     yield;
     assert {:phase 1} Inv(ghostLock, currsize, newsize);
@@ -64,134 +67,127 @@ requires {:phase 1} xls' == mapconstbool(true);
     }
 }
 
-procedure {:yields} {:phase 1} Thread({:linear "tid"} tid': X)
-requires {:phase 1} tid' != nil;
+procedure {:yields} {:phase 1} Thread({:cnst "tid"} tid: X)
+requires {:phase 1} tid != nil;
 requires {:phase 1} Inv(ghostLock, currsize, newsize);
 {
     var start, size, bytesRead: int;
-    var {:linear "tid"} tid: X;
 
-    tid := tid';
     havoc start, size;
     assume (0 <= start && 0 <= size);
     call bytesRead := Read(tid, start, size);
 }
 
-procedure {:yields} {:phase 1} Read({:linear "tid"} tid': X, start : int, size : int) returns (bytesRead : int)
-requires {:phase 1} tid' != nil;
+procedure {:yields} {:phase 1} Read({:cnst "tid"} tid: X, start : int, size : int) returns (bytesRead : int)
+requires {:phase 1} tid != nil;
 requires {:phase 1} 0 <= start && 0 <= size;
 requires {:phase 1} Inv(ghostLock, currsize, newsize);
 ensures {:phase 1} 0 <= bytesRead && bytesRead <= size;
 {
     var i, tmp: int;
-    var {:linear "tid"} tid: X;
-    tid := tid';
 
-    par  tid := YieldToReadCache(tid);
+    par YieldToReadCache(tid);
     bytesRead := size;
-    call tid := acquire(tid);
-    call tid, i := ReadCurrsize(tid);
-    call tid, tmp := ReadNewsize(tid);
+    call acquire(tid);
+    call i := ReadCurrsize(tid);
+    call tmp := ReadNewsize(tid);
     if (start + size <= i) {
-        call tid := release(tid); 
+        call release(tid); 
     	goto COPY_TO_BUFFER;
     } else if (tmp > i) {
         bytesRead := if (start <= i) then (i - start) else 0;
-    	call tid := release(tid); 
+    	call release(tid); 
 	goto COPY_TO_BUFFER;
     } else {
-        call tid := WriteNewsize(tid, start + size);
-    	call tid := release(tid); 
+        call WriteNewsize(tid, start + size);
+    	call release(tid); 
 	goto READ_DEVICE;
     }
 
 READ_DEVICE:
-    par  tid := YieldToWriteCache(tid);
-    call tid := WriteCache(tid, start + size);
-    par  tid := YieldToWriteCache(tid);
-    call tid := acquire(tid);
-    call tid, tmp := ReadNewsize(tid);
-    call tid := WriteCurrsize(tid, tmp);
-    call tid := release(tid);
+    par YieldToWriteCache(tid);
+    call WriteCache(tid, start + size);
+    par YieldToWriteCache(tid);
+    call acquire(tid);
+    call tmp := ReadNewsize(tid);
+    call WriteCurrsize(tid, tmp);
+    call release(tid);
 
 COPY_TO_BUFFER:
-    par tid := YieldToReadCache(tid);
-    call tid := ReadCache(tid, start, bytesRead);
+    par YieldToReadCache(tid);
+    call ReadCache(tid, start, bytesRead);
 }
 
-procedure {:yields} {:phase 1} WriteCache({:linear "tid"} tid': X, index: int) returns ({:linear "tid"} tid: X)
+procedure {:yields} {:phase 1} WriteCache({:cnst "tid"} tid: X, index: int)
 requires {:phase 1} Inv(ghostLock, currsize, newsize);
-requires {:phase 1} ghostLock == tid' && tid' != nil;
-ensures {:phase 1} tid == tid' && ghostLock == tid;
+requires {:phase 1} ghostLock == tid && tid != nil;
+ensures {:phase 1} ghostLock == tid;
 ensures {:phase 1} Inv(ghostLock, currsize, newsize) && old(currsize) == currsize && old(newsize) == newsize;
 {
     var j: int;
-    tid := tid';
 
-    par tid := YieldToWriteCache(tid);
-    call tid, j := ReadCurrsize(tid);
+    par YieldToWriteCache(tid);
+    call j := ReadCurrsize(tid);
     while (j < index)
-    invariant {:phase 1} ghostLock == tid && currsize <= j && tid == tid';
+    invariant {:phase 1} ghostLock == tid && currsize <= j && tid == tid;
     invariant {:phase 1} Inv(ghostLock, currsize, newsize) && old(currsize) == currsize && old(newsize) == newsize;
     {
-        par tid := YieldToWriteCache(tid);
-        call tid := WriteCacheEntry(tid, j);
+        par YieldToWriteCache(tid);
+        call WriteCacheEntry(tid, j);
 	j := j + 1;
     }
-    par tid := YieldToWriteCache(tid);
+    par YieldToWriteCache(tid);
 }
 
-procedure {:yields} {:phase 1} ReadCache({:linear "tid"} tid': X, start: int, bytesRead: int) returns ({:linear "tid"} tid: X)
+procedure {:yields} {:phase 1} ReadCache({:cnst "tid"} tid: X, start: int, bytesRead: int)
 requires {:phase 1} Inv(ghostLock, currsize, newsize);
-requires {:phase 1} tid' != nil;
+requires {:phase 1} tid != nil;
 requires {:phase 1} 0 <= start && 0 <= bytesRead;
 requires {:phase 1} (bytesRead == 0 || start + bytesRead <= currsize);
-ensures {:phase 1} tid == tid';
 ensures {:phase 1} Inv(ghostLock, currsize, newsize);
 {
     var j: int;
-    tid := tid';
 
-    par tid := YieldToReadCache(tid);
+    par YieldToReadCache(tid);
 
     j := 0;
     while(j < bytesRead)
     invariant {:phase 1} 0 <= j;
     invariant {:phase 1} bytesRead == 0 || start + bytesRead <= currsize; 
-    invariant {:phase 1} Inv(ghostLock, currsize, newsize) && tid == tid';
+    invariant {:phase 1} Inv(ghostLock, currsize, newsize);
     {
 	assert {:phase 1} start + j < currsize;
-        call tid := ReadCacheEntry(tid, start + j);
+        call ReadCacheEntry(tid, start + j);
         j := j + 1;
-	par tid := YieldToReadCache(tid);
+	par YieldToReadCache(tid);
     }
 
-    par tid := YieldToReadCache(tid);
+    par YieldToReadCache(tid);
 }
 
-procedure {:yields} {:phase 0,1} Init({:linear "tid"} xls':[X]bool) returns ({:linear "tid"} xls:[X]bool);
-ensures {:atomic} |{ A: assert xls' == mapconstbool(true); xls := xls'; currsize := 0; newsize := 0; lock := nil; ghostLock := nil; return true; }|;
+procedure {:yields} {:phase 0,1} Init({:cnst "tid"} xls:[X]bool);
+ensures {:atomic} |{ A: assert xls == mapconstbool(true); currsize := 0; newsize := 0; lock := nil; ghostLock := nil; return true; }|;
 
-procedure {:yields} {:phase 0,1} ReadCurrsize({:linear "tid"} tid': X) returns ({:linear "tid"} tid: X, val: int);
-ensures {:right} |{A: assert tid' != nil; assert lock == tid' || ghostLock == tid'; tid := tid'; val := currsize; return true; }|;
+procedure {:yields} {:phase 0,1} ReadCurrsize({:cnst "tid"} tid: X) returns (val: int);
+ensures {:right} |{A: assert tid != nil; assert lock == tid || ghostLock == tid; val := currsize; return true; }|;
 
-procedure {:yields} {:phase 0,1} ReadNewsize({:linear "tid"} tid': X) returns ({:linear "tid"} tid: X, val: int);
-ensures {:right} |{A: assert tid' != nil; assert lock == tid' || ghostLock == tid'; tid := tid'; val := newsize; return true; }|;
+procedure {:yields} {:phase 0,1} ReadNewsize({:cnst "tid"} tid: X) returns (val: int);
+ensures {:right} |{A: assert tid != nil; assert lock == tid || ghostLock == tid; val := newsize; return true; }|;
 
-procedure {:yields} {:phase 0,1} WriteNewsize({:linear "tid"} tid': X, val: int) returns ({:linear "tid"} tid: X);
-ensures {:atomic} |{A: assert tid' != nil; assert lock == tid' && ghostLock == nil; tid := tid'; newsize := val; ghostLock := tid; return true; }|;
+procedure {:yields} {:phase 0,1} WriteNewsize({:cnst "tid"} tid: X, val: int);
+ensures {:atomic} |{A: assert tid != nil; assert lock == tid && ghostLock == nil; newsize := val; ghostLock := tid; return true; }|;
 
-procedure {:yields} {:phase 0,1} WriteCurrsize({:linear "tid"} tid': X, val: int) returns ({:linear "tid"} tid: X);
-ensures {:atomic} |{A: assert tid' != nil; assert lock == tid' && ghostLock == tid'; tid := tid'; currsize := val; ghostLock := nil; return true; }|;
+procedure {:yields} {:phase 0,1} WriteCurrsize({:cnst "tid"} tid: X, val: int);
+ensures {:atomic} |{A: assert tid != nil; assert lock == tid && ghostLock == tid; currsize := val; ghostLock := nil; return true; }|;
 
-procedure {:yields} {:phase 0,1} ReadCacheEntry({:linear "tid"} tid': X, index: int) returns ({:linear "tid"} tid: X);
-ensures {:atomic} |{ A: assert 0 <= index && index < currsize; tid := tid'; return true; }|;
+procedure {:yields} {:phase 0,1} ReadCacheEntry({:cnst "tid"} tid: X, index: int);
+ensures {:atomic} |{ A: assert 0 <= index && index < currsize; return true; }|;
 
-procedure {:yields} {:phase 0,1} WriteCacheEntry({:linear "tid"} tid': X, index: int) returns ({:linear "tid"} tid: X);
-ensures {:right} |{ A: assert tid' != nil; assert currsize <= index && ghostLock == tid'; tid := tid'; return true; }|;
+procedure {:yields} {:phase 0,1} WriteCacheEntry({:cnst "tid"} tid: X, index: int);
+ensures {:right} |{ A: assert tid != nil; assert currsize <= index && ghostLock == tid; return true; }|;
 
-procedure {:yields} {:phase 0,1} acquire({:linear "tid"} tid': X) returns ({:linear "tid"} tid: X);
-ensures {:right} |{ A: assert tid' != nil; tid := tid'; assume lock == nil; lock := tid; return true; }|;
+procedure {:yields} {:phase 0,1} acquire({:cnst "tid"} tid: X);
+ensures {:right} |{ A: assert tid != nil; assume lock == nil; lock := tid; return true; }|;
 
-procedure {:yields} {:phase 0,1} release({:linear "tid"} tid': X) returns ({:linear "tid"} tid: X);
-ensures {:left} |{ A: assert tid' != nil; assert lock == tid'; tid := tid'; lock := nil; return true; }|;
+procedure {:yields} {:phase 0,1} release({:cnst "tid"} tid: X);
+ensures {:left} |{ A: assert tid != nil; assert lock == tid; lock := nil; return true; }|;
